04Stack/StackConversion.thy
@@ -2,68 +2,68 @@ theory StackConversion
   imports Stack
 begin
 
-fun unwind' :: "frame list \<Rightarrow> expr\<^sub>d \<Rightarrow> expr\<^sub>d" where
+fun unwind' :: "frame\<^sub>k list \<Rightarrow> expr\<^sub>d \<Rightarrow> expr\<^sub>d" where
   "unwind' [] e = e"
-| "unwind' (FApp1 e\<^sub>2 # s) e = unwind' s (App\<^sub>d e e\<^sub>2)"
-| "unwind' (FApp2 e\<^sub>1 # s) e = unwind' s (App\<^sub>d e\<^sub>1 e)"
-| "unwind' (FReturn # s) e = unwind' s e"
+| "unwind' (FApp1\<^sub>k e\<^sub>2 # s) e = unwind' s (App\<^sub>d e e\<^sub>2)"
+| "unwind' (FApp2\<^sub>k e\<^sub>1 # s) e = unwind' s (App\<^sub>d e\<^sub>1 e)"
+| "unwind' (FReturn\<^sub>k # s) e = unwind' s e"
 
-primrec unwind :: "stack_state \<Rightarrow> expr\<^sub>d" where
-  "unwind (SS b s e) = unwind' s e"
+primrec unwind :: "state\<^sub>k \<Rightarrow> expr\<^sub>d" where
+  "unwind (S\<^sub>k b s e) = unwind' s e"
 
-lemma [simp]: "s : t' \<rightarrow> t \<Longrightarrow> [] \<turnstile>\<^sub>d e : t' \<Longrightarrow> [] \<turnstile>\<^sub>d unwind' s e : t"
-  by (induction s t' t arbitrary: e rule: typecheck_stack.induct) simp_all
+lemma [simp]: "s :\<^sub>k t' \<rightarrow> t \<Longrightarrow> [] \<turnstile>\<^sub>d e : t' \<Longrightarrow> [] \<turnstile>\<^sub>d unwind' s e : t"
+  by (induction s t' t arbitrary: e rule: typing_stack\<^sub>k.induct) simp_all
 
-theorem typesafed [simp]: "\<Sigma> :\<^sub>s t \<Longrightarrow> [] \<turnstile>\<^sub>d unwind \<Sigma> : t"
-  by (induction \<Sigma> t rule: typecheck_stack_state.induct) simp_all
+theorem typesafed [simp]: "\<Sigma> :\<^sub>k t \<Longrightarrow> [] \<turnstile>\<^sub>d unwind \<Sigma> : t"
+  by (induction \<Sigma> t rule: typing_state\<^sub>k.induct) simp_all
 
-lemma [simp]: "s : t' \<rightarrow> t \<Longrightarrow> e \<leadsto>\<^sub>d e' \<Longrightarrow> unwind' s e \<leadsto>\<^sub>d unwind' s e'"
-  by (induction s t' t arbitrary: e e' rule: typecheck_stack.induct) simp_all
+lemma [simp]: "s :\<^sub>k t' \<rightarrow> t \<Longrightarrow> e \<leadsto>\<^sub>d e' \<Longrightarrow> unwind' s e \<leadsto>\<^sub>d unwind' s e'"
+  by (induction s t' t arbitrary: e e' rule: typing_stack\<^sub>k.induct) simp_all
 
-theorem correctd: "\<Sigma> \<leadsto>\<^sub>s \<Sigma>' \<Longrightarrow> \<Sigma> :\<^sub>s t \<Longrightarrow> iter (\<leadsto>\<^sub>d) (unwind \<Sigma>) (unwind \<Sigma>')"
-proof (induction \<Sigma> \<Sigma>' rule: evals.induct)
-  case (evs_app3 t\<^sub>1 e\<^sub>1 s e\<^sub>2)
-  then obtain t\<^sub>2 where "(s : t\<^sub>2 \<rightarrow> t) \<and> value\<^sub>d e\<^sub>2" by blast
+theorem correctd: "\<Sigma> \<leadsto>\<^sub>k \<Sigma>' \<Longrightarrow> \<Sigma> :\<^sub>k t \<Longrightarrow> iter (\<leadsto>\<^sub>d) (unwind \<Sigma>) (unwind \<Sigma>')"
+proof (induction \<Sigma> \<Sigma>' rule: eval\<^sub>k.induct)
+  case (ev\<^sub>k_app3 t\<^sub>1 e\<^sub>1 s e\<^sub>2)
+  then obtain t\<^sub>2 where "(s :\<^sub>k t\<^sub>2 \<rightarrow> t) \<and> value\<^sub>d e\<^sub>2" by blast
   moreover hence "App\<^sub>d (Lam\<^sub>d t\<^sub>1 e\<^sub>1) e\<^sub>2 \<leadsto>\<^sub>d subst\<^sub>d 0 e\<^sub>2 e\<^sub>1" by simp
   ultimately have "unwind' s (App\<^sub>d (Lam\<^sub>d t\<^sub>1 e\<^sub>1) e\<^sub>2) \<leadsto>\<^sub>d unwind' s (subst\<^sub>d 0 e\<^sub>2 e\<^sub>1)" by auto
   thus ?case by simp
 qed simp_all
 
-primrec all_returns :: "frame list \<Rightarrow> bool" where
+primrec all_returns :: "frame\<^sub>k list \<Rightarrow> bool" where
   "all_returns [] = True"
-| "all_returns (r # rs) = (r = FReturn \<and> all_returns rs)"
+| "all_returns (r # rs) = (r = FReturn\<^sub>k \<and> all_returns rs)"
 
 lemma unwind_returns [elim]: "all_returns sr \<Longrightarrow> unwind' sr e = e"
   by (induction sr) (simp_all add: all_returns_def)
 
-lemma [dest]: "FApp1 e # sr : t' \<rightarrow> t \<Longrightarrow> all_returns sr \<Longrightarrow> 
+lemma [dest]: "FApp1\<^sub>k e # sr :\<^sub>k t' \<rightarrow> t \<Longrightarrow> all_returns sr \<Longrightarrow> 
     (\<And>t\<^sub>1. t' = Arrow t\<^sub>1 t \<Longrightarrow> [] \<turnstile>\<^sub>d e : t\<^sub>1 \<Longrightarrow> P) \<Longrightarrow> P"
   by (induction sr) fastforce+
 
-lemma [dest]: "FApp2 e # sr : t' \<rightarrow> t \<Longrightarrow> all_returns sr \<Longrightarrow> 
+lemma [dest]: "FApp2\<^sub>k e # sr :\<^sub>k t' \<rightarrow> t \<Longrightarrow> all_returns sr \<Longrightarrow> 
     ([] \<turnstile>\<^sub>d e : Arrow t' t \<Longrightarrow> value\<^sub>d e \<Longrightarrow> P) \<Longrightarrow> P"
   by (induction sr) fastforce+
 
-lemma [dest]: "sr @ s : t' \<rightarrow> t \<Longrightarrow> all_returns sr \<Longrightarrow> (s : t' \<rightarrow> t \<Longrightarrow> P) \<Longrightarrow> P"
+lemma [dest]: "sr @ s :\<^sub>k t' \<rightarrow> t \<Longrightarrow> all_returns sr \<Longrightarrow> (s :\<^sub>k t' \<rightarrow> t \<Longrightarrow> P) \<Longrightarrow> P"
   by (induction sr) fastforce+
 
 lemma [dest]: "App\<^sub>d e\<^sub>1 e\<^sub>2 = unwind' s e \<Longrightarrow> (all_returns s \<and> e = App\<^sub>d e\<^sub>1 e\<^sub>2) \<or> 
-  (\<exists>s' sr. all_returns sr \<and> ((s = s' @ FApp1 e\<^sub>2 # sr \<and> e\<^sub>1 = unwind' s' e) \<or> 
-    (s = s' @ FApp2 e\<^sub>1 # sr \<and> e\<^sub>2 = unwind' s' e)))"
+  (\<exists>s' sr. all_returns sr \<and> ((s = s' @ FApp1\<^sub>k e\<^sub>2 # sr \<and> e\<^sub>1 = unwind' s' e) \<or> 
+    (s = s' @ FApp2\<^sub>k e\<^sub>1 # sr \<and> e\<^sub>2 = unwind' s' e)))"
 proof (induction s e rule: unwind'.induct)
   case (2 e\<^sub>2' s e)
   thus ?case
   proof (cases "all_returns s \<and> App\<^sub>d e e\<^sub>2' = App\<^sub>d e\<^sub>1 e\<^sub>2")
     case False
-    with 2 obtain s' sr where S: "all_returns sr \<and> ((s = s' @ FApp1 e\<^sub>2 # sr \<and> 
-      e\<^sub>1 = unwind' s' (App\<^sub>d e e\<^sub>2')) \<or> (s = s' @ FApp2 e\<^sub>1 # sr \<and> e\<^sub>2 = unwind' s' (App\<^sub>d e e\<^sub>2')))" 
+    with 2 obtain s' sr where S: "all_returns sr \<and> ((s = s' @ FApp1\<^sub>k e\<^sub>2 # sr \<and> 
+      e\<^sub>1 = unwind' s' (App\<^sub>d e e\<^sub>2')) \<or> (s = s' @ FApp2\<^sub>k e\<^sub>1 # sr \<and> e\<^sub>2 = unwind' s' (App\<^sub>d e e\<^sub>2')))" 
         by fastforce
     thus ?thesis
-    proof (cases "s = s' @ FApp1 e\<^sub>2 # sr \<and> e\<^sub>1 = unwind' s' (App\<^sub>d e e\<^sub>2')")
+    proof (cases "s = s' @ FApp1\<^sub>k e\<^sub>2 # sr \<and> e\<^sub>1 = unwind' s' (App\<^sub>d e e\<^sub>2')")
       case False
-      with S have "all_returns sr \<and> s = s' @ FApp2 e\<^sub>1 # sr \<and> e\<^sub>2 = unwind' s' (App\<^sub>d e e\<^sub>2')" by simp
-      moreover hence "FApp1 e\<^sub>2' # s' @ FApp2 e\<^sub>1 # sr = (FApp1 e\<^sub>2' # s') @ FApp2 e\<^sub>1 # sr \<and> 
-        unwind' s' (App\<^sub>d e e\<^sub>2') = unwind' (FApp1 e\<^sub>2' # s') e" by simp
+      with S have "all_returns sr \<and> s = s' @ FApp2\<^sub>k e\<^sub>1 # sr \<and> e\<^sub>2 = unwind' s' (App\<^sub>d e e\<^sub>2')" by simp
+      moreover hence "FApp1\<^sub>k e\<^sub>2' # s' @ FApp2\<^sub>k e\<^sub>1 # sr = (FApp1\<^sub>k e\<^sub>2' # s') @ FApp2\<^sub>k e\<^sub>1 # sr \<and> 
+        unwind' s' (App\<^sub>d e e\<^sub>2') = unwind' (FApp1\<^sub>k e\<^sub>2' # s') e" by simp
       ultimately show ?thesis by blast
     qed fastforce+
   qed fastforce+
@@ -72,15 +72,15 @@ next
   thus ?case
   proof (cases "all_returns s \<and> App\<^sub>d e\<^sub>1' e = App\<^sub>d e\<^sub>1 e\<^sub>2")
     case False
-    with 3 obtain s' sr where S: "all_returns sr \<and> ((s = s' @ FApp1 e\<^sub>2 # sr \<and> 
-      e\<^sub>1 = unwind' s' (App\<^sub>d e\<^sub>1' e)) \<or> (s = s' @ FApp2 e\<^sub>1 # sr \<and> e\<^sub>2 = unwind' s' (App\<^sub>d e\<^sub>1' e)))" 
+    with 3 obtain s' sr where S: "all_returns sr \<and> ((s = s' @ FApp1\<^sub>k e\<^sub>2 # sr \<and> 
+      e\<^sub>1 = unwind' s' (App\<^sub>d e\<^sub>1' e)) \<or> (s = s' @ FApp2\<^sub>k e\<^sub>1 # sr \<and> e\<^sub>2 = unwind' s' (App\<^sub>d e\<^sub>1' e)))" 
         by fastforce
     thus ?thesis
-    proof (cases "s = s' @ FApp1 e\<^sub>2 # sr \<and> e\<^sub>1 = unwind' s' (App\<^sub>d e\<^sub>1' e)")
+    proof (cases "s = s' @ FApp1\<^sub>k e\<^sub>2 # sr \<and> e\<^sub>1 = unwind' s' (App\<^sub>d e\<^sub>1' e)")
       case False
-      with S have "all_returns sr \<and> s = s' @ FApp2 e\<^sub>1 # sr \<and> e\<^sub>2 = unwind' s' (App\<^sub>d e\<^sub>1' e)" by simp
-      moreover hence "FApp2 e\<^sub>1' # s' @ FApp2 e\<^sub>1 # sr = (FApp2 e\<^sub>1' # s') @ FApp2 e\<^sub>1 # sr \<and> 
-        e\<^sub>2 = unwind' (FApp2 e\<^sub>1' # s') e" by simp
+      with S have "all_returns sr \<and> s = s' @ FApp2\<^sub>k e\<^sub>1 # sr \<and> e\<^sub>2 = unwind' s' (App\<^sub>d e\<^sub>1' e)" by simp
+      moreover hence "FApp2\<^sub>k e\<^sub>1' # s' @ FApp2\<^sub>k e\<^sub>1 # sr = (FApp2\<^sub>k e\<^sub>1' # s') @ FApp2\<^sub>k e\<^sub>1 # sr \<and> 
+        e\<^sub>2 = unwind' (FApp2\<^sub>k e\<^sub>1' # s') e" by simp
       ultimately show ?thesis by blast
     qed fastforce+
   qed fastforce+
@@ -89,14 +89,14 @@ next
   thus ?case
   proof (cases "all_returns s \<and> e = App\<^sub>d e\<^sub>1 e\<^sub>2")
     case False
-    with 4 obtain s' sr where S: "all_returns sr \<and> ((s = s' @ FApp1 e\<^sub>2 # sr \<and> e\<^sub>1 = unwind' s' e) \<or> 
-      (s = s' @ FApp2 e\<^sub>1 # sr \<and> e\<^sub>2 = unwind' s' e))" by fastforce
+    with 4 obtain s' sr where S: "all_returns sr \<and> ((s = s' @ FApp1\<^sub>k e\<^sub>2 # sr \<and> e\<^sub>1 = unwind' s' e) \<or> 
+      (s = s' @ FApp2\<^sub>k e\<^sub>1 # sr \<and> e\<^sub>2 = unwind' s' e))" by fastforce
     thus ?thesis
-    proof (cases "s = s' @ FApp1 e\<^sub>2 # sr \<and> e\<^sub>1 = unwind' s' e")
+    proof (cases "s = s' @ FApp1\<^sub>k e\<^sub>2 # sr \<and> e\<^sub>1 = unwind' s' e")
       case False
-      with S have "all_returns sr \<and> s = s' @ FApp2 e\<^sub>1 # sr \<and> e\<^sub>2 = unwind' s' e" by simp
-      moreover hence "FReturn # s' @ FApp2 e\<^sub>1 # sr = (FReturn # s') @ FApp2 e\<^sub>1 # sr \<and> 
-        e\<^sub>2 = unwind' (FReturn # s') e" by simp
+      with S have "all_returns sr \<and> s = s' @ FApp2\<^sub>k e\<^sub>1 # sr \<and> e\<^sub>2 = unwind' s' e" by simp
+      moreover hence "FReturn\<^sub>k # s' @ FApp2\<^sub>k e\<^sub>1 # sr = (FReturn\<^sub>k # s') @ FApp2\<^sub>k e\<^sub>1 # sr \<and> 
+        e\<^sub>2 = unwind' (FReturn\<^sub>k # s') e" by simp
       ultimately show ?thesis by blast
     qed fastforce+
   qed fastforce+
@@ -105,27 +105,27 @@ qed simp_all
 lemma [simp]: "value\<^sub>d v \<Longrightarrow> v = unwind' s e \<Longrightarrow> all_returns s \<and> e = v"
   by (induction s e rule: unwind'.induct) simp_all
 
-lemma [simp]: "value\<^sub>d v \<Longrightarrow> v = unwind \<Sigma> \<Longrightarrow> \<exists>b s. \<Sigma> = SS b s v \<and> all_returns s"
+lemma [simp]: "value\<^sub>d v \<Longrightarrow> v = unwind \<Sigma> \<Longrightarrow> \<exists>b s. \<Sigma> = S\<^sub>k b s v \<and> all_returns s"
   by (induction \<Sigma>) simp_all
 
-lemma [simp]: "all_returns sr \<Longrightarrow> unwind' (s @ FApp1 e\<^sub>2 # sr) e = App\<^sub>d (unwind' s e) e\<^sub>2"
+lemma [simp]: "all_returns sr \<Longrightarrow> unwind' (s @ FApp1\<^sub>k e\<^sub>2 # sr) e = App\<^sub>d (unwind' s e) e\<^sub>2"
   by (induction s e rule: unwind'.induct) auto
 
-lemma [simp]: "all_returns sr \<Longrightarrow> unwind' (s @ FApp2 e\<^sub>1 # sr) e = App\<^sub>d e\<^sub>1 (unwind' s e)"
+lemma [simp]: "all_returns sr \<Longrightarrow> unwind' (s @ FApp2\<^sub>k e\<^sub>1 # sr) e = App\<^sub>d e\<^sub>1 (unwind' s e)"
   by (induction s e rule: unwind'.induct) auto
 
-lemma eval_returns [simp]: "all_returns sr \<Longrightarrow> value\<^sub>d v \<Longrightarrow> iter (\<leadsto>\<^sub>s) (SS b (sr @ s) v) (SS True s v)"
+lemma eval_returns [simp]: "all_returns sr \<Longrightarrow> value\<^sub>d v \<Longrightarrow> iter (\<leadsto>\<^sub>k) (S\<^sub>k b (sr @ s) v) (S\<^sub>k True s v)"
 proof (induction sr arbitrary: b)
   case (Cons a sr)
-  hence "iter (\<leadsto>\<^sub>s) (SS b (FReturn # sr @ s) v) (SS True (FReturn # sr @ s) v)" by simp
-  hence "iter (\<leadsto>\<^sub>s) (SS b (FReturn # sr @ s) v) (SS True (sr @ s) v)" by simp
-  moreover from Cons have "iter (\<leadsto>\<^sub>s) (SS True (sr @ s) v) (SS True s v)" by simp
-  ultimately have "iter (\<leadsto>\<^sub>s) (SS b (FReturn # sr @ s) v) (SS True s v)" by (metis iter_append)
+  hence "iter (\<leadsto>\<^sub>k) (S\<^sub>k b (FReturn\<^sub>k # sr @ s) v) (S\<^sub>k True (FReturn\<^sub>k # sr @ s) v)" by simp
+  hence "iter (\<leadsto>\<^sub>k) (S\<^sub>k b (FReturn\<^sub>k # sr @ s) v) (S\<^sub>k True (sr @ s) v)" by simp
+  moreover from Cons have "iter (\<leadsto>\<^sub>k) (S\<^sub>k True (sr @ s) v) (S\<^sub>k True s v)" by simp
+  ultimately have "iter (\<leadsto>\<^sub>k) (S\<^sub>k b (FReturn\<^sub>k # sr @ s) v) (S\<^sub>k True s v)" by (metis iter_append)
   with Cons show ?case by simp
 qed simp_all
 
-lemma [simp]: "unwind' s e \<leadsto>\<^sub>d e' \<Longrightarrow> s : t' \<rightarrow> t \<Longrightarrow> [] \<turnstile>\<^sub>d e : tt \<Longrightarrow> (b \<Longrightarrow> value\<^sub>d e) \<Longrightarrow>
-  \<exists>b' s' e''. iter (\<leadsto>\<^sub>s) (SS b s e) (SS b' s' e'') \<and> e' = unwind' s' e''"
+lemma [simp]: "unwind' s e \<leadsto>\<^sub>d e' \<Longrightarrow> s :\<^sub>k t' \<rightarrow> t \<Longrightarrow> [] \<turnstile>\<^sub>d e : tt \<Longrightarrow> (b \<Longrightarrow> value\<^sub>d e) \<Longrightarrow>
+  \<exists>b' s' e''. iter (\<leadsto>\<^sub>k) (S\<^sub>k b s e) (S\<^sub>k b' s' e'') \<and> e' = unwind' s' e''"
 proof (induction "unwind' s e" e' arbitrary: b s e t tt rule: eval\<^sub>d.induct)
   case (ev\<^sub>d_app1 e\<^sub>1 e\<^sub>1' e\<^sub>2)
   thus ?case
@@ -133,33 +133,33 @@ proof (induction "unwind' s e" e' arbitrary: b s e t tt rule: eval\<^sub>d.induc
     case True
     with ev\<^sub>d_app1 have B: "\<not>b" by (cases b) simp_all
     from ev\<^sub>d_app1 True obtain t\<^sub>1 where T1: "([] \<turnstile>\<^sub>d e\<^sub>1 : Arrow t\<^sub>1 tt) \<and> ([] \<turnstile>\<^sub>d e\<^sub>2 : t\<^sub>1)" by blast
-    have "[] : t' \<rightarrow> t'" by simp
-    with ev\<^sub>d_app1 B T1 obtain b' s' e'' where E: "iter (\<leadsto>\<^sub>s) (SS False [] e\<^sub>1) (SS b' s' e'') \<and> 
+    have "[] :\<^sub>k t' \<rightarrow> t'" by simp
+    with ev\<^sub>d_app1 B T1 obtain b' s' e'' where E: "iter (\<leadsto>\<^sub>k) (S\<^sub>k False [] e\<^sub>1) (S\<^sub>k b' s' e'') \<and> 
       e\<^sub>1' = unwind' s' e''" by fastforce
-    hence "iter (\<leadsto>\<^sub>s) (SS False ([] @ FApp1 e\<^sub>2 # s) e\<^sub>1) (SS b' (s' @ FApp1 e\<^sub>2 # s) e'')" 
-      by (metis eval_under)
-    hence "iter (\<leadsto>\<^sub>s) (SS False (FApp1 e\<^sub>2 # s) e\<^sub>1) (SS b' (s' @ FApp1 e\<^sub>2 # s) e'')" by simp
-    hence "iter (\<leadsto>\<^sub>s) (SS False s (App\<^sub>d e\<^sub>1 e\<^sub>2)) (SS b' (s' @ FApp1 e\<^sub>2 # s) e'')" 
-      by (metis evs_app1 iter_step)
+    hence "iter (\<leadsto>\<^sub>k) (S\<^sub>k False ([] @ FApp1\<^sub>k e\<^sub>2 # s) e\<^sub>1) (S\<^sub>k b' (s' @ FApp1\<^sub>k e\<^sub>2 # s) e'')" 
+      by (metis eval\<^sub>k_under_iter)
+    hence "iter (\<leadsto>\<^sub>k) (S\<^sub>k False (FApp1\<^sub>k e\<^sub>2 # s) e\<^sub>1) (S\<^sub>k b' (s' @ FApp1\<^sub>k e\<^sub>2 # s) e'')" by simp
+    hence "iter (\<leadsto>\<^sub>k) (S\<^sub>k False s (App\<^sub>d e\<^sub>1 e\<^sub>2)) (S\<^sub>k b' (s' @ FApp1\<^sub>k e\<^sub>2 # s) e'')" 
+      by (metis ev\<^sub>k_app1 iter_step)
     with True B E show ?thesis by fastforce
   next
     case False
     with ev\<^sub>d_app1 obtain s' sr where S: "all_returns sr \<and> 
-      ((s = s' @ FApp1 e\<^sub>2 # sr \<and> e\<^sub>1 = unwind' s' e) \<or> 
-        (s = s' @ FApp2 e\<^sub>1 # sr \<and> e\<^sub>2 = unwind' s' e))" by fast
+      ((s = s' @ FApp1\<^sub>k e\<^sub>2 # sr \<and> e\<^sub>1 = unwind' s' e) \<or> 
+        (s = s' @ FApp2\<^sub>k e\<^sub>1 # sr \<and> e\<^sub>2 = unwind' s' e))" by fast
     thus ?thesis
-    proof (cases "s = s' @ FApp1 e\<^sub>2 # sr \<and> e\<^sub>1 = unwind' s' e")
+    proof (cases "s = s' @ FApp1\<^sub>k e\<^sub>2 # sr \<and> e\<^sub>1 = unwind' s' e")
       case True
-      with ev\<^sub>d_app1 obtain t'' where "(s' : t' \<rightarrow> t'') \<and> (FApp1 e\<^sub>2 # sr : t'' \<rightarrow> t)" by fastforce
-      with ev\<^sub>d_app1 True obtain b' ss' e'' where S': "iter (\<leadsto>\<^sub>s) (SS b s' e) (SS b' ss' e'') \<and> 
+      with ev\<^sub>d_app1 obtain t'' where "(s' :\<^sub>k t' \<rightarrow> t'') \<and> (FApp1\<^sub>k e\<^sub>2 # sr :\<^sub>k t'' \<rightarrow> t)" by fastforce
+      with ev\<^sub>d_app1 True obtain b' ss' e'' where S': "iter (\<leadsto>\<^sub>k) (S\<^sub>k b s' e) (S\<^sub>k b' ss' e'') \<and> 
         e\<^sub>1' = unwind' ss' e''" by blast
-      hence X: "iter (\<leadsto>\<^sub>s) (SS b (s' @ FApp1 e\<^sub>2 # sr) e) (SS b' (ss' @ FApp1 e\<^sub>2 # sr) e'')" by simp
-      from S S' have "App\<^sub>d e\<^sub>1' e\<^sub>2 = unwind' (ss' @ FApp1 e\<^sub>2 # sr) e''" by simp
+      hence X: "iter (\<leadsto>\<^sub>k) (S\<^sub>k b (s' @ FApp1\<^sub>k e\<^sub>2 # sr) e) (S\<^sub>k b' (ss' @ FApp1\<^sub>k e\<^sub>2 # sr) e'')" by simp
+      from S S' have "App\<^sub>d e\<^sub>1' e\<^sub>2 = unwind' (ss' @ FApp1\<^sub>k e\<^sub>2 # sr) e''" by simp
       with True X show ?thesis by blast
     next
       case False
-      with S have "s = s' @ FApp2 e\<^sub>1 # sr \<and> e\<^sub>2 = unwind' s' e" by simp
-      with ev\<^sub>d_app1 obtain t\<^sub>1 where "(s' : t' \<rightarrow> t\<^sub>1) \<and> (FApp2 e\<^sub>1 # sr : t\<^sub>1 \<rightarrow> t)" by fastforce
+      with S have "s = s' @ FApp2\<^sub>k e\<^sub>1 # sr \<and> e\<^sub>2 = unwind' s' e" by simp
+      with ev\<^sub>d_app1 obtain t\<^sub>1 where "(s' :\<^sub>k t' \<rightarrow> t\<^sub>1) \<and> (FApp2\<^sub>k e\<^sub>1 # sr :\<^sub>k t\<^sub>1 \<rightarrow> t)" by fastforce
       with S have "([] \<turnstile>\<^sub>d e\<^sub>1 : Arrow t\<^sub>1 t) \<and> value\<^sub>d e\<^sub>1" by fastforce
       with ev\<^sub>d_app1 show ?thesis by (metis val_no_eval\<^sub>d)
     qed
@@ -171,50 +171,50 @@ next
     case True
     with ev\<^sub>d_app2 have B: "\<not>b" by (cases b) simp_all
     from ev\<^sub>d_app2 True obtain t\<^sub>1 where T: "([] \<turnstile>\<^sub>d e\<^sub>1 : Arrow t\<^sub>1 tt) \<and> ([] \<turnstile>\<^sub>d e\<^sub>2 : t\<^sub>1)" by blast
-    with ev\<^sub>d_app2 B obtain b' s' e'' where E: "iter (\<leadsto>\<^sub>s) (SS False [] e\<^sub>2) (SS b' s' e'') \<and> 
-      e\<^sub>2' = unwind' s' e''" by (metis unwind'.simps(1) tcs_nil)
-    hence "iter (\<leadsto>\<^sub>s) (SS False (FApp2 e\<^sub>1 # s) e\<^sub>2) (SS b' (s' @ FApp2 e\<^sub>1 # s) e'')" 
-      by (metis eval_under append_Nil)
-    moreover have "SS False s (App\<^sub>d e\<^sub>1 e\<^sub>2) \<leadsto>\<^sub>s SS False (FApp1 e\<^sub>2 # s) e\<^sub>1" by simp
-    moreover from ev\<^sub>d_app2 have "iter (\<leadsto>\<^sub>s) (SS False (FApp1 e\<^sub>2 # s) e\<^sub>1) (SS True (FApp1 e\<^sub>2 # s) e\<^sub>1)" 
+    with ev\<^sub>d_app2 B obtain b' s' e'' where E: "iter (\<leadsto>\<^sub>k) (S\<^sub>k False [] e\<^sub>2) (S\<^sub>k b' s' e'') \<and> 
+      e\<^sub>2' = unwind' s' e''" by (metis unwind'.simps(1) tcs\<^sub>k_nil)
+    hence "iter (\<leadsto>\<^sub>k) (S\<^sub>k False (FApp2\<^sub>k e\<^sub>1 # s) e\<^sub>2) (S\<^sub>k b' (s' @ FApp2\<^sub>k e\<^sub>1 # s) e'')" 
+      by (metis eval\<^sub>k_under_iter append_Nil)
+    moreover have "S\<^sub>k False s (App\<^sub>d e\<^sub>1 e\<^sub>2) \<leadsto>\<^sub>k S\<^sub>k False (FApp1\<^sub>k e\<^sub>2 # s) e\<^sub>1" by simp
+    moreover from ev\<^sub>d_app2 have "iter (\<leadsto>\<^sub>k) (S\<^sub>k False (FApp1\<^sub>k e\<^sub>2 # s) e\<^sub>1) (S\<^sub>k True (FApp1\<^sub>k e\<^sub>2 # s) e\<^sub>1)" 
       by simp
-    moreover have "SS True (FApp1 e\<^sub>2 # s) e\<^sub>1 \<leadsto>\<^sub>s SS False (FApp2 e\<^sub>1 # s) e\<^sub>2" by simp
-    ultimately have "iter (\<leadsto>\<^sub>s) (SS False s (App\<^sub>d e\<^sub>1 e\<^sub>2)) (SS b' (s' @ FApp2 e\<^sub>1 # s) e'')" 
+    moreover have "S\<^sub>k True (FApp1\<^sub>k e\<^sub>2 # s) e\<^sub>1 \<leadsto>\<^sub>k S\<^sub>k False (FApp2\<^sub>k e\<^sub>1 # s) e\<^sub>2" by simp
+    ultimately have "iter (\<leadsto>\<^sub>k) (S\<^sub>k False s (App\<^sub>d e\<^sub>1 e\<^sub>2)) (S\<^sub>k b' (s' @ FApp2\<^sub>k e\<^sub>1 # s) e'')" 
       by (metis iter_step iter_append)
     with True B E show ?thesis by fastforce
   next
     case False
     with ev\<^sub>d_app2 obtain s' sr where S: "all_returns sr \<and> 
-      ((s = s' @ FApp1 e\<^sub>2 # sr \<and> e\<^sub>1 = unwind' s' e) \<or> 
-        (s = s' @ FApp2 e\<^sub>1 # sr \<and> e\<^sub>2 = unwind' s' e))" by blast
+      ((s = s' @ FApp1\<^sub>k e\<^sub>2 # sr \<and> e\<^sub>1 = unwind' s' e) \<or> 
+        (s = s' @ FApp2\<^sub>k e\<^sub>1 # sr \<and> e\<^sub>2 = unwind' s' e))" by blast
     thus ?thesis
-    proof (cases "s = s' @ FApp1 e\<^sub>2 # sr \<and> e\<^sub>1 = unwind' s' e")
+    proof (cases "s = s' @ FApp1\<^sub>k e\<^sub>2 # sr \<and> e\<^sub>1 = unwind' s' e")
       case True
       with ev\<^sub>d_app2 have S': "all_returns s' \<and> e = e\<^sub>1" by simp 
       with ev\<^sub>d_app2 True S obtain t\<^sub>1 where T: "t' = Arrow t\<^sub>1 t \<and> [] \<turnstile>\<^sub>d e\<^sub>2 : t\<^sub>1" by blast
       have X: "e\<^sub>2 = unwind' [] e\<^sub>2" by simp
-      have E: "[] : t' \<rightarrow> t'" by simp
+      have E: "[] :\<^sub>k t' \<rightarrow> t'" by simp
       have "False \<Longrightarrow> value\<^sub>d e\<^sub>2" by simp
-      with ev\<^sub>d_app2 T X E obtain b'' s'' e'' where E: "iter (\<leadsto>\<^sub>s) (SS False [] e\<^sub>2) (SS b'' s'' e'') \<and> 
+      with ev\<^sub>d_app2 T X E obtain b'' s'' e'' where E: "iter (\<leadsto>\<^sub>k) (S\<^sub>k False [] e\<^sub>2) (S\<^sub>k b'' s'' e'') \<and> 
         e\<^sub>2' = unwind' s'' e''" by blast
-      hence "iter (\<leadsto>\<^sub>s) (SS False (FApp2 e\<^sub>1 # sr) e\<^sub>2) (SS b'' (s'' @ FApp2 e\<^sub>1 # sr) e'')" 
-        using eval_under by fastforce
-      moreover from ev\<^sub>d_app2 have "SS True (FApp1 e\<^sub>2 # sr) e\<^sub>1 \<leadsto>\<^sub>s SS False (FApp2 e\<^sub>1 # sr) e\<^sub>2" by simp
-      moreover from ev\<^sub>d_app2 S' have "iter (\<leadsto>\<^sub>s) (SS True (s' @ FApp1 e\<^sub>2 # sr) e\<^sub>1) 
-        (SS True (FApp1 e\<^sub>2 # sr) e\<^sub>1)" by simp
-      moreover from ev\<^sub>d_app2 S' have "iter (\<leadsto>\<^sub>s) (SS b (s' @ FApp1 e\<^sub>2 # sr) e\<^sub>1) 
-        (SS True (s' @ FApp1 e\<^sub>2 # sr) e\<^sub>1)" by simp
-      ultimately have Y: "iter (\<leadsto>\<^sub>s) (SS b (s' @ FApp1 e\<^sub>2 # sr) e\<^sub>1) 
-        (SS b'' (s'' @ FApp2 e\<^sub>1 # sr) e'')" by (metis iter_step iter_append)
-      from S E have "App\<^sub>d e\<^sub>1 e\<^sub>2' = unwind' (s'' @ FApp2 e\<^sub>1 # sr) e''" by simp
+      hence "iter (\<leadsto>\<^sub>k) (S\<^sub>k False (FApp2\<^sub>k e\<^sub>1 # sr) e\<^sub>2) (S\<^sub>k b'' (s'' @ FApp2\<^sub>k e\<^sub>1 # sr) e'')" 
+        using eval\<^sub>k_under_iter by fastforce
+      moreover from ev\<^sub>d_app2 have "S\<^sub>k True (FApp1\<^sub>k e\<^sub>2 # sr) e\<^sub>1 \<leadsto>\<^sub>k S\<^sub>k False (FApp2\<^sub>k e\<^sub>1 # sr) e\<^sub>2" by simp
+      moreover from ev\<^sub>d_app2 S' have "iter (\<leadsto>\<^sub>k) (S\<^sub>k True (s' @ FApp1\<^sub>k e\<^sub>2 # sr) e\<^sub>1) 
+        (S\<^sub>k True (FApp1\<^sub>k e\<^sub>2 # sr) e\<^sub>1)" by simp
+      moreover from ev\<^sub>d_app2 S' have "iter (\<leadsto>\<^sub>k) (S\<^sub>k b (s' @ FApp1\<^sub>k e\<^sub>2 # sr) e\<^sub>1) 
+        (S\<^sub>k True (s' @ FApp1\<^sub>k e\<^sub>2 # sr) e\<^sub>1)" by simp
+      ultimately have Y: "iter (\<leadsto>\<^sub>k) (S\<^sub>k b (s' @ FApp1\<^sub>k e\<^sub>2 # sr) e\<^sub>1) 
+        (S\<^sub>k b'' (s'' @ FApp2\<^sub>k e\<^sub>1 # sr) e'')" by (metis iter_step iter_append)
+      from S E have "App\<^sub>d e\<^sub>1 e\<^sub>2' = unwind' (s'' @ FApp2\<^sub>k e\<^sub>1 # sr) e''" by simp
       with True S' Y show ?thesis by auto
     next
       case False
-      with S have S': "s = s' @ FApp2 e\<^sub>1 # sr \<and> e\<^sub>2 = unwind' s' e" by simp
-      with ev\<^sub>d_app2 obtain t\<^sub>1 where "(s' : t' \<rightarrow> t\<^sub>1) \<and> (FApp2 e\<^sub>1 # sr : t\<^sub>1 \<rightarrow> t)" by fastforce
-      with ev\<^sub>d_app2 S' obtain b'' s'' e'' where E: "iter (\<leadsto>\<^sub>s) (SS b s' e) (SS b'' s'' e'') \<and> 
+      with S have S': "s = s' @ FApp2\<^sub>k e\<^sub>1 # sr \<and> e\<^sub>2 = unwind' s' e" by simp
+      with ev\<^sub>d_app2 obtain t\<^sub>1 where "(s' :\<^sub>k t' \<rightarrow> t\<^sub>1) \<and> (FApp2\<^sub>k e\<^sub>1 # sr :\<^sub>k t\<^sub>1 \<rightarrow> t)" by fastforce
+      with ev\<^sub>d_app2 S' obtain b'' s'' e'' where E: "iter (\<leadsto>\<^sub>k) (S\<^sub>k b s' e) (S\<^sub>k b'' s'' e'') \<and> 
         e\<^sub>2' = unwind' s'' e''" by blast
-      hence "iter (\<leadsto>\<^sub>s) (SS b (s' @ FApp2 e\<^sub>1 # sr) e) (SS b'' (s'' @ FApp2 e\<^sub>1 # sr) e'')" by simp
+      hence "iter (\<leadsto>\<^sub>k) (S\<^sub>k b (s' @ FApp2\<^sub>k e\<^sub>1 # sr) e) (S\<^sub>k b'' (s'' @ FApp2\<^sub>k e\<^sub>1 # sr) e'')" by simp
       with S S' E show ?thesis by fastforce
     qed
   qed
@@ -224,92 +224,92 @@ next
   proof (cases "all_returns s \<and> e = App\<^sub>d (Lam\<^sub>d t\<^sub>1 e\<^sub>1) e\<^sub>2")
     case True
     with ev\<^sub>d_app3 have B: "\<not>b" by (cases b) simp_all
-    have "SS False s (App\<^sub>d (Lam\<^sub>d t\<^sub>1 e\<^sub>1) e\<^sub>2) \<leadsto>\<^sub>s SS False (FApp1 e\<^sub>2 # s) (Lam\<^sub>d t\<^sub>1 e\<^sub>1)" by simp
-    moreover have "SS False (FApp1 e\<^sub>2 # s) (Lam\<^sub>d t\<^sub>1 e\<^sub>1) \<leadsto>\<^sub>s SS True  (FApp1 e\<^sub>2 # s) (Lam\<^sub>d t\<^sub>1 e\<^sub>1)" 
+    have "S\<^sub>k False s (App\<^sub>d (Lam\<^sub>d t\<^sub>1 e\<^sub>1) e\<^sub>2) \<leadsto>\<^sub>k S\<^sub>k False (FApp1\<^sub>k e\<^sub>2 # s) (Lam\<^sub>d t\<^sub>1 e\<^sub>1)" by simp
+    moreover have "S\<^sub>k False (FApp1\<^sub>k e\<^sub>2 # s) (Lam\<^sub>d t\<^sub>1 e\<^sub>1) \<leadsto>\<^sub>k S\<^sub>k True  (FApp1\<^sub>k e\<^sub>2 # s) (Lam\<^sub>d t\<^sub>1 e\<^sub>1)" 
       by simp
-    moreover have "SS True (FApp1 e\<^sub>2 # s) (Lam\<^sub>d t\<^sub>1 e\<^sub>1) \<leadsto>\<^sub>s SS False (FApp2 (Lam\<^sub>d t\<^sub>1 e\<^sub>1) # s) e\<^sub>2" 
+    moreover have "S\<^sub>k True (FApp1\<^sub>k e\<^sub>2 # s) (Lam\<^sub>d t\<^sub>1 e\<^sub>1) \<leadsto>\<^sub>k S\<^sub>k False (FApp2\<^sub>k (Lam\<^sub>d t\<^sub>1 e\<^sub>1) # s) e\<^sub>2" 
       by simp
-    moreover from ev\<^sub>d_app3 have "iter (\<leadsto>\<^sub>s) (SS False (FApp2 (Lam\<^sub>d t\<^sub>1 e\<^sub>1) # s) e\<^sub>2) 
-      (SS True (FApp2 (Lam\<^sub>d t\<^sub>1 e\<^sub>1) # s) e\<^sub>2)" by simp
-    moreover have "SS True (FApp2 (Lam\<^sub>d t\<^sub>1 e\<^sub>1) # s) e\<^sub>2 \<leadsto>\<^sub>s SS False (FReturn # s) (subst\<^sub>d 0 e\<^sub>2 e\<^sub>1)" 
+    moreover from ev\<^sub>d_app3 have "iter (\<leadsto>\<^sub>k) (S\<^sub>k False (FApp2\<^sub>k (Lam\<^sub>d t\<^sub>1 e\<^sub>1) # s) e\<^sub>2) 
+      (S\<^sub>k True (FApp2\<^sub>k (Lam\<^sub>d t\<^sub>1 e\<^sub>1) # s) e\<^sub>2)" by simp
+    moreover have "S\<^sub>k True (FApp2\<^sub>k (Lam\<^sub>d t\<^sub>1 e\<^sub>1) # s) e\<^sub>2 \<leadsto>\<^sub>k S\<^sub>k False (FReturn\<^sub>k # s) (subst\<^sub>d 0 e\<^sub>2 e\<^sub>1)" 
       by simp
-    ultimately have X: "iter (\<leadsto>\<^sub>s) (SS False s (App\<^sub>d (Lam\<^sub>d t\<^sub>1 e\<^sub>1) e\<^sub>2)) 
-      (SS False (FReturn # s) (subst\<^sub>d 0 e\<^sub>2 e\<^sub>1))" by (metis iter_step iter_refl iter_append)
-    from True have "subst\<^sub>d 0 e\<^sub>2 e\<^sub>1 = unwind' (FReturn # s) (subst\<^sub>d 0 e\<^sub>2 e\<^sub>1)"
+    ultimately have X: "iter (\<leadsto>\<^sub>k) (S\<^sub>k False s (App\<^sub>d (Lam\<^sub>d t\<^sub>1 e\<^sub>1) e\<^sub>2)) 
+      (S\<^sub>k False (FReturn\<^sub>k # s) (subst\<^sub>d 0 e\<^sub>2 e\<^sub>1))" by (metis iter_step iter_refl iter_append)
+    from True have "subst\<^sub>d 0 e\<^sub>2 e\<^sub>1 = unwind' (FReturn\<^sub>k # s) (subst\<^sub>d 0 e\<^sub>2 e\<^sub>1)"
       using unwind_returns by simp
     with True B X show ?thesis by fastforce
   next
     case False
     with ev\<^sub>d_app3 obtain s' sr where S: "all_returns sr \<and> 
-      ((s = s' @ FApp1 e\<^sub>2 # sr \<and> Lam\<^sub>d t\<^sub>1 e\<^sub>1 = unwind' s' e) \<or> 
-        (s = s' @ FApp2 (Lam\<^sub>d t\<^sub>1 e\<^sub>1) # sr \<and> e\<^sub>2 = unwind' s' e))" by blast
+      ((s = s' @ FApp1\<^sub>k e\<^sub>2 # sr \<and> Lam\<^sub>d t\<^sub>1 e\<^sub>1 = unwind' s' e) \<or> 
+        (s = s' @ FApp2\<^sub>k (Lam\<^sub>d t\<^sub>1 e\<^sub>1) # sr \<and> e\<^sub>2 = unwind' s' e))" by blast
     thus ?thesis
-    proof (cases "s = s' @ FApp1 e\<^sub>2 # sr \<and> Lam\<^sub>d t\<^sub>1 e\<^sub>1 = unwind' s' e")
+    proof (cases "s = s' @ FApp1\<^sub>k e\<^sub>2 # sr \<and> Lam\<^sub>d t\<^sub>1 e\<^sub>1 = unwind' s' e")
       case True
       moreover have "value\<^sub>d (Lam\<^sub>d t\<^sub>1 e\<^sub>1)" by simp
       ultimately have S': "all_returns s' \<and> e = Lam\<^sub>d t\<^sub>1 e\<^sub>1" by simp
-      have "SS True (FApp1 e\<^sub>2 # sr) (Lam\<^sub>d t\<^sub>1 e\<^sub>1) \<leadsto>\<^sub>s SS False (FApp2 (Lam\<^sub>d t\<^sub>1 e\<^sub>1) # sr) e\<^sub>2" by simp
-      moreover from ev\<^sub>d_app3 have "iter (\<leadsto>\<^sub>s) (SS False (FApp2 (Lam\<^sub>d t\<^sub>1 e\<^sub>1) # sr) e\<^sub>2) 
-        (SS True (FApp2 (Lam\<^sub>d t\<^sub>1 e\<^sub>1) # sr) e\<^sub>2)" by simp
-      moreover from ev\<^sub>d_app3 have "SS True (FApp2 (Lam\<^sub>d t\<^sub>1 e\<^sub>1) # sr) e\<^sub>2 \<leadsto>\<^sub>s 
-        SS False (FReturn # sr) (subst\<^sub>d 0 e\<^sub>2 e\<^sub>1)" by simp
-      moreover from S' have "iter (\<leadsto>\<^sub>s) (SS True (s' @ FApp1 e\<^sub>2 # sr) (Lam\<^sub>d t\<^sub>1 e\<^sub>1)) 
-        (SS True (FApp1 e\<^sub>2 # sr) (Lam\<^sub>d t\<^sub>1 e\<^sub>1))" by simp
-      moreover have "iter (\<leadsto>\<^sub>s) (SS b (s' @ FApp1 e\<^sub>2 # sr) (Lam\<^sub>d t\<^sub>1 e\<^sub>1)) 
-        (SS True (s' @ FApp1 e\<^sub>2 # sr) (Lam\<^sub>d t\<^sub>1 e\<^sub>1))" by simp
-      ultimately have X: "iter (\<leadsto>\<^sub>s) (SS b (s' @ FApp1 e\<^sub>2 # sr) (Lam\<^sub>d t\<^sub>1 e\<^sub>1)) 
-        (SS False (FReturn # sr) (subst\<^sub>d 0 e\<^sub>2 e\<^sub>1))" by (metis iter_step iter_refl iter_append)
-      from S True have "subst\<^sub>d 0 e\<^sub>2 e\<^sub>1 = unwind' (FReturn # sr) (subst\<^sub>d 0 e\<^sub>2 e\<^sub>1)" 
+      have "S\<^sub>k True (FApp1\<^sub>k e\<^sub>2 # sr) (Lam\<^sub>d t\<^sub>1 e\<^sub>1) \<leadsto>\<^sub>k S\<^sub>k False (FApp2\<^sub>k (Lam\<^sub>d t\<^sub>1 e\<^sub>1) # sr) e\<^sub>2" by simp
+      moreover from ev\<^sub>d_app3 have "iter (\<leadsto>\<^sub>k) (S\<^sub>k False (FApp2\<^sub>k (Lam\<^sub>d t\<^sub>1 e\<^sub>1) # sr) e\<^sub>2) 
+        (S\<^sub>k True (FApp2\<^sub>k (Lam\<^sub>d t\<^sub>1 e\<^sub>1) # sr) e\<^sub>2)" by simp
+      moreover from ev\<^sub>d_app3 have "S\<^sub>k True (FApp2\<^sub>k (Lam\<^sub>d t\<^sub>1 e\<^sub>1) # sr) e\<^sub>2 \<leadsto>\<^sub>k 
+        S\<^sub>k False (FReturn\<^sub>k # sr) (subst\<^sub>d 0 e\<^sub>2 e\<^sub>1)" by simp
+      moreover from S' have "iter (\<leadsto>\<^sub>k) (S\<^sub>k True (s' @ FApp1\<^sub>k e\<^sub>2 # sr) (Lam\<^sub>d t\<^sub>1 e\<^sub>1)) 
+        (S\<^sub>k True (FApp1\<^sub>k e\<^sub>2 # sr) (Lam\<^sub>d t\<^sub>1 e\<^sub>1))" by simp
+      moreover have "iter (\<leadsto>\<^sub>k) (S\<^sub>k b (s' @ FApp1\<^sub>k e\<^sub>2 # sr) (Lam\<^sub>d t\<^sub>1 e\<^sub>1)) 
+        (S\<^sub>k True (s' @ FApp1\<^sub>k e\<^sub>2 # sr) (Lam\<^sub>d t\<^sub>1 e\<^sub>1))" by simp
+      ultimately have X: "iter (\<leadsto>\<^sub>k) (S\<^sub>k b (s' @ FApp1\<^sub>k e\<^sub>2 # sr) (Lam\<^sub>d t\<^sub>1 e\<^sub>1)) 
+        (S\<^sub>k False (FReturn\<^sub>k # sr) (subst\<^sub>d 0 e\<^sub>2 e\<^sub>1))" by (metis iter_step iter_refl iter_append)
+      from S True have "subst\<^sub>d 0 e\<^sub>2 e\<^sub>1 = unwind' (FReturn\<^sub>k # sr) (subst\<^sub>d 0 e\<^sub>2 e\<^sub>1)" 
         using unwind_returns by simp
       with True S' X show ?thesis by fastforce
     next
       case False
       with S ev\<^sub>d_app3 have S': "all_returns s' \<and> e = e\<^sub>2" by simp
-      from ev\<^sub>d_app3 have "SS True (FApp2 (Lam\<^sub>d t\<^sub>1 e\<^sub>1) # sr) e\<^sub>2 \<leadsto>\<^sub>s 
-        SS False (FReturn # sr) (subst\<^sub>d 0 e\<^sub>2 e\<^sub>1)" by simp
-      hence "iter (\<leadsto>\<^sub>s) (SS True (FApp2 (Lam\<^sub>d t\<^sub>1 e\<^sub>1) # sr) e\<^sub>2) 
-        (SS False (FReturn # sr) (subst\<^sub>d 0 e\<^sub>2 e\<^sub>1))" by (metis iter_step iter_refl)
-      moreover from ev\<^sub>d_app3 S' have "iter (\<leadsto>\<^sub>s) (SS True (s' @ FApp2 (Lam\<^sub>d t\<^sub>1 e\<^sub>1) # sr) e\<^sub>2) 
-        (SS True (FApp2 (Lam\<^sub>d t\<^sub>1 e\<^sub>1) # sr) e\<^sub>2)" by simp
-      moreover from ev\<^sub>d_app3 have "iter (\<leadsto>\<^sub>s) (SS b (s' @ FApp2 (Lam\<^sub>d t\<^sub>1 e\<^sub>1) # sr) e\<^sub>2) 
-        (SS True (s' @ FApp2 (Lam\<^sub>d t\<^sub>1 e\<^sub>1) # sr) e\<^sub>2)" by simp
-      ultimately have X: "iter (\<leadsto>\<^sub>s) (SS b (s' @ FApp2 (Lam\<^sub>d t\<^sub>1 e\<^sub>1) # sr) e\<^sub>2) 
-        (SS False (FReturn # sr) (subst\<^sub>d 0 e\<^sub>2 e\<^sub>1))" by (metis iter_append)
-      from S have "subst\<^sub>d 0 e\<^sub>2 e\<^sub>1 = unwind' (FReturn # sr) (subst\<^sub>d 0 e\<^sub>2 e\<^sub>1)" 
+      from ev\<^sub>d_app3 have "S\<^sub>k True (FApp2\<^sub>k (Lam\<^sub>d t\<^sub>1 e\<^sub>1) # sr) e\<^sub>2 \<leadsto>\<^sub>k 
+        S\<^sub>k False (FReturn\<^sub>k # sr) (subst\<^sub>d 0 e\<^sub>2 e\<^sub>1)" by simp
+      hence "iter (\<leadsto>\<^sub>k) (S\<^sub>k True (FApp2\<^sub>k (Lam\<^sub>d t\<^sub>1 e\<^sub>1) # sr) e\<^sub>2) 
+        (S\<^sub>k False (FReturn\<^sub>k # sr) (subst\<^sub>d 0 e\<^sub>2 e\<^sub>1))" by (metis iter_step iter_refl)
+      moreover from ev\<^sub>d_app3 S' have "iter (\<leadsto>\<^sub>k) (S\<^sub>k True (s' @ FApp2\<^sub>k (Lam\<^sub>d t\<^sub>1 e\<^sub>1) # sr) e\<^sub>2) 
+        (S\<^sub>k True (FApp2\<^sub>k (Lam\<^sub>d t\<^sub>1 e\<^sub>1) # sr) e\<^sub>2)" by simp
+      moreover from ev\<^sub>d_app3 have "iter (\<leadsto>\<^sub>k) (S\<^sub>k b (s' @ FApp2\<^sub>k (Lam\<^sub>d t\<^sub>1 e\<^sub>1) # sr) e\<^sub>2) 
+        (S\<^sub>k True (s' @ FApp2\<^sub>k (Lam\<^sub>d t\<^sub>1 e\<^sub>1) # sr) e\<^sub>2)" by simp
+      ultimately have X: "iter (\<leadsto>\<^sub>k) (S\<^sub>k b (s' @ FApp2\<^sub>k (Lam\<^sub>d t\<^sub>1 e\<^sub>1) # sr) e\<^sub>2) 
+        (S\<^sub>k False (FReturn\<^sub>k # sr) (subst\<^sub>d 0 e\<^sub>2 e\<^sub>1))" by (metis iter_append)
+      from S have "subst\<^sub>d 0 e\<^sub>2 e\<^sub>1 = unwind' (FReturn\<^sub>k # sr) (subst\<^sub>d 0 e\<^sub>2 e\<^sub>1)" 
         using unwind_returns by simp
       with S False S' X show ?thesis by metis
     qed
   qed
 qed
 
-theorem completed [simp]: "\<Sigma> :\<^sub>s t \<Longrightarrow> unwind \<Sigma> \<leadsto>\<^sub>d e' \<Longrightarrow> \<exists>\<Sigma>'. iter (\<leadsto>\<^sub>s) \<Sigma> \<Sigma>' \<and> e' = unwind \<Sigma>'"
-proof (induction \<Sigma> t rule: typecheck_stack_state.induct)
-  case (tcs_state s t' t e b)
-  then obtain b' s' e'' where "iter (\<leadsto>\<^sub>s) (SS b s e) (SS b' s' e'') \<and> e' = unwind' s' e''" by fastforce
+theorem completed [simp]: "\<Sigma> :\<^sub>k t \<Longrightarrow> unwind \<Sigma> \<leadsto>\<^sub>d e' \<Longrightarrow> \<exists>\<Sigma>'. iter (\<leadsto>\<^sub>k) \<Sigma> \<Sigma>' \<and> e' = unwind \<Sigma>'"
+proof (induction \<Sigma> t rule: typing_state\<^sub>k.induct)
+  case (tc_state\<^sub>k s t' t e b)
+  then obtain b' s' e'' where "iter (\<leadsto>\<^sub>k) (S\<^sub>k b s e) (S\<^sub>k b' s' e'') \<and> e' = unwind' s' e''" by fastforce
   thus ?case by fastforce
 qed
 
-lemma [simp]: "iter (\<leadsto>\<^sub>d) (unwind \<Sigma>) e' \<Longrightarrow> \<Sigma> :\<^sub>s t \<Longrightarrow> \<exists>\<Sigma>'. iter (\<leadsto>\<^sub>s) \<Sigma> \<Sigma>' \<and> e' = unwind \<Sigma>'"
+lemma [simp]: "iter (\<leadsto>\<^sub>d) (unwind \<Sigma>) e' \<Longrightarrow> \<Sigma> :\<^sub>k t \<Longrightarrow> \<exists>\<Sigma>'. iter (\<leadsto>\<^sub>k) \<Sigma> \<Sigma>' \<and> e' = unwind \<Sigma>'"
 proof (induction "unwind \<Sigma>" e' arbitrary: \<Sigma> rule: iter.induct)
   case (iter_step e' e'')
-  moreover then obtain \<Sigma>' where S: "iter (\<leadsto>\<^sub>s) \<Sigma> \<Sigma>' \<and> e' = unwind \<Sigma>'" by fastforce
-  moreover with iter_step have "\<Sigma>' :\<^sub>s t" by fastforce
-  ultimately obtain \<Sigma>'' where "iter (\<leadsto>\<^sub>s) \<Sigma>' \<Sigma>'' \<and> e'' = unwind \<Sigma>''" by fastforce
-  with S have "iter (\<leadsto>\<^sub>s) \<Sigma> \<Sigma>'' \<and> e'' = unwind \<Sigma>''" by (metis iter_append)
+  moreover then obtain \<Sigma>' where S: "iter (\<leadsto>\<^sub>k) \<Sigma> \<Sigma>' \<and> e' = unwind \<Sigma>'" by fastforce
+  moreover with iter_step have "\<Sigma>' :\<^sub>k t" by fastforce
+  ultimately obtain \<Sigma>'' where "iter (\<leadsto>\<^sub>k) \<Sigma>' \<Sigma>'' \<and> e'' = unwind \<Sigma>''" by fastforce
+  with S have "iter (\<leadsto>\<^sub>k) \<Sigma> \<Sigma>'' \<and> e'' = unwind \<Sigma>''" by (metis iter_append)
   then show ?case by fastforce
 qed force+
 
 lemma [simp]: "iter (\<leadsto>\<^sub>d) e v \<Longrightarrow> [] \<turnstile>\<^sub>d e : t \<Longrightarrow> value\<^sub>d v \<Longrightarrow> 
-  iter (\<leadsto>\<^sub>s) (SS False [FReturn] e) (SS True [] v)"
+  iter (\<leadsto>\<^sub>k) (S\<^sub>k False [FReturn\<^sub>k] e) (S\<^sub>k True [] v)"
 proof -
   assume "[] \<turnstile>\<^sub>d e : t"
-  hence "SS False [FReturn] e :\<^sub>s t" by (metis tcs_nil tcs_cons_ret tcs_state)
+  hence "S\<^sub>k False [FReturn\<^sub>k] e :\<^sub>k t" by (metis tcs\<^sub>k_nil tcs\<^sub>k_cons_ret tc_state\<^sub>k)
   moreover assume "iter (\<leadsto>\<^sub>d) e v"
-  ultimately obtain \<Sigma>' where S: "iter (\<leadsto>\<^sub>s) (SS False [FReturn] e) \<Sigma>' \<and> v = unwind \<Sigma>'" by fastforce
+  ultimately obtain \<Sigma>' where S: "iter (\<leadsto>\<^sub>k) (S\<^sub>k False [FReturn\<^sub>k] e) \<Sigma>' \<and> v = unwind \<Sigma>'" by fastforce
   moreover assume V: "value\<^sub>d v"
-  ultimately obtain b sr where "\<Sigma>' = SS b (sr @ []) v \<and> all_returns sr" by fastforce
-  moreover with V have "iter (\<leadsto>\<^sub>s) \<Sigma>' (SS True [] v)" by (metis eval_returns)
-  with S show "iter (\<leadsto>\<^sub>s) (SS False [FReturn] e) (SS True [] v)" by (metis iter_append)
+  ultimately obtain b sr where "\<Sigma>' = S\<^sub>k b (sr @ []) v \<and> all_returns sr" by fastforce
+  moreover with V have "iter (\<leadsto>\<^sub>k) \<Sigma>' (S\<^sub>k True [] v)" by (metis eval_returns)
+  with S show "iter (\<leadsto>\<^sub>k) (S\<^sub>k False [FReturn\<^sub>k] e) (S\<^sub>k True [] v)" by (metis iter_append)
 qed
 
 end
